fairneris/examples/retransmit_example_adequacy.v
@@ -1,0 +1,193 @@
+From stdpp Require Import list fin_maps.
+From iris.proofmode Require Import proofmode.
+From trillium.program_logic Require Import ectx_lifting.
+From fairneris Require Import fairness.
+From fairneris.examples Require Import retransmit_model_progress_ltl.
+From fairneris.aneris_lang Require Import aneris_lang.
+From fairneris.aneris_lang.state_interp Require Import state_interp state_interp_events.
+From fairneris.aneris_lang.program_logic Require Import aneris_weakestpre.
+From fairneris Require Import retransmit_example adequacy.
+From fairneris.lib Require Import singletons.
+
+Definition initial_state shA shB :=
+  ([mkExpr ipA (Aprog shA); mkExpr ipB (Bprog shB)],
+     {| state_heaps := {[ipA:=∅; ipB:=∅]};
+        state_sockets := {[ipA := {[shA := (sA, [])]};
+                           ipB := {[shB := (sB, [])]}]};
+        state_ms := ∅; |}).
+
+Definition initial_model_state : retransmit_state :=
+  (retransmit_model_base.Start, ∅, {[saA := []; saB := []]}).
+
+Lemma retransmit_continued_simulation shA shB :
+  fairly_terminating localeB (initial_state shA shB).
+Proof.
+  assert (anerisPreG retransmit_fair_model (anerisΣ retransmit_fair_model)) as HPreG.
+  { apply _. }
+  eapply (simulation_adequacy_fair_termination_multiple {[saA;saB]} NotStuck _ _ initial_model_state);
+    [| |simpl; lia|set_solver|..|done|]=> /=.
+  { intros ℓ ζ Hmatch Henabled. rewrite /role_enabled_model in Henabled. simpl.
+    assert (ℓ = Arole ∨ ℓ = Brole) as [Heq|Heq] by set_solver; simplify_eq.
+    - assert (ζ = ("0.0.0.0", 0%nat)) as ->.
+      { rewrite /roles_match /locale_retransmit_role in Hmatch.
+        by repeat case_match; simplify_eq. }
+      eexists _. simpl. done.
+    - assert (ζ = ("0.0.0.1", 0%nat)) as ->.
+      { rewrite /roles_match /locale_retransmit_role in Hmatch.
+        by repeat case_match; simplify_eq. }
+      eexists _. simpl. done. }
+  { rewrite /config_state_valid. simpl. split; [done|].
+    rewrite /model_state_socket_coh.
+    intros.
+    (* OBS: Might be able to make this simpler with a total lookup *)
+    rewrite insert_union_singleton_l in H.
+    (* rewrite lookup_union in H. *)
+    apply lookup_union_Some in H; [|apply map_disjoint_dom; set_solver].
+    destruct H as [H|H].
+    - destruct (decide (ip = ipA)) as [->|Hneq]; last first.
+      { by rewrite lookup_insert_ne in H. }
+      rewrite lookup_insert in H.
+      simplify_eq.
+      destruct (decide (sh = shA)) as [->|Hneq]; last first.
+      { by rewrite lookup_insert_ne in H0. }
+      rewrite lookup_insert in H0.
+      simplify_eq.
+      assert (sa = saA) as -> by set_solver.
+      set_solver.
+    - destruct (decide (ip = ipB)) as [->|Hneq]; last first.
+      { by rewrite lookup_insert_ne in H. }
+      rewrite lookup_insert in H.
+      simplify_eq.
+      destruct (decide (sh = shB)) as [->|Hneq]; last first.
+      { by rewrite lookup_insert_ne in H0. }
+      rewrite lookup_insert in H0.
+      simplify_eq.
+      assert (sa = saB) as -> by set_solver.
+      set_solver. }
+  { intros ip ps HPs Sn Hip p Hps.
+    intros sh skt a r Hsh Hskt.
+    intros <-.
+    assert (ports_in_use {[ipA := {[shA := (sA, [])]}; ipB := {[shB := (sB, [])]}]} = {[saA; saB]}) as Heq.
+    { rewrite /ports_in_use.
+      rewrite map_fold_insert_L; [by rewrite !map_fold_singleton| |set_solver].
+      intros j1 j2 z1 z2 y Hneq Hz1 Hz2.
+      rewrite insert_union_singleton_l in Hz1.
+      apply lookup_union_Some in Hz1; last first.
+      { apply map_disjoint_dom. clear. set_solver. }
+      rewrite insert_union_singleton_l in Hz2.
+      apply lookup_union_Some in Hz2; last first.
+      { apply map_disjoint_dom. clear. set_solver. }
+      destruct Hz1 as [Hz1|Hz1], Hz2 as [Hz2|Hz2].
+      - apply lookup_singleton_Some in Hz1 as [<- <-].
+        apply lookup_singleton_Some in Hz2 as [<- <-].
+        done.
+      - apply lookup_singleton_Some in Hz1 as [<- <-].
+        apply lookup_singleton_Some in Hz2 as [<- <-].
+        rewrite !map_fold_singleton=> /=.
+        clear. rewrite !union_empty_r_L !union_assoc_L. set_solver.
+      - apply lookup_singleton_Some in Hz1 as [<- <-].
+        apply lookup_singleton_Some in Hz2 as [<- <-].
+        rewrite !map_fold_singleton=> /=.
+        clear. rewrite !union_empty_r_L !union_assoc_L. set_solver.
+      - apply lookup_singleton_Some in Hz1 as [<- <-].
+        apply lookup_singleton_Some in Hz2 as [<- <-].
+        rewrite !map_fold_singleton=> /=.
+        clear. rewrite !union_empty_r_L !union_assoc_L. set_solver. }
+    rewrite Heq in HPs. clear Heq.
+    rewrite difference_diag_L in HPs. done. }
+  { intros ip Sn Hip.
+    intros sh [skt bs] Hsh.
+    rewrite insert_union_singleton_l in Hip.
+    apply lookup_union_Some in Hip; [|apply map_disjoint_dom; set_solver].
+    destruct Hip as [Hip|Hip].
+    - destruct (decide (ip = ipA)) as [->|Hneq]; last first.
+      { by rewrite lookup_insert_ne in Hip. }
+      rewrite lookup_insert in Hip.
+      simplify_eq.
+      destruct (decide (sh = shA)) as [->|Hneq]; last first.
+      { by rewrite lookup_insert_ne in Hsh. }
+      rewrite lookup_insert in Hsh.
+      simplify_eq. done.
+    - destruct (decide (ip = ipB)) as [->|Hneq]; last first.
+      { by rewrite lookup_insert_ne in Hip. }
+      rewrite lookup_insert in Hip.
+      simplify_eq.
+      destruct (decide (sh = shB)) as [->|Hneq]; last first.
+      { by rewrite lookup_insert_ne in Hsh. }
+      rewrite lookup_insert in Hsh.
+      simplify_eq. done. }
+  { intros ip Sn Hip sh sh' skt skt' bs bs' Hsh Hsh' Hskt Heq.
+    rewrite insert_union_singleton_l in Hip.
+    apply lookup_union_Some in Hip; [|apply map_disjoint_dom; set_solver].
+    destruct Hip as [Hip|Hip].
+    - destruct (decide (ip = ipA)) as [->|Hneq]; last first.
+      { by rewrite lookup_insert_ne in Hip. }
+      rewrite lookup_insert in Hip.
+      simplify_eq.
+      destruct (decide (sh = shA)) as [->|Hneq]; last first.
+      { by rewrite lookup_insert_ne in Hsh. }
+      rewrite lookup_insert in Hsh.
+      destruct (decide (sh' = shA)) as [->|Hneq]; last first.
+      { by rewrite lookup_insert_ne in Hsh'. }
+      rewrite lookup_insert in Hsh'.
+      done.
+    - destruct (decide (ip = ipB)) as [->|Hneq]; last first.
+      { by rewrite lookup_insert_ne in Hip. }
+      rewrite lookup_insert in Hip.
+      simplify_eq.
+      destruct (decide (sh = shB)) as [->|Hneq]; last first.
+      { by rewrite lookup_insert_ne in Hsh. }
+      rewrite lookup_insert in Hsh.
+      destruct (decide (sh' = shB)) as [->|Hneq]; last first.
+      { by rewrite lookup_insert_ne in Hsh'. }
+      rewrite lookup_insert in Hsh'.
+      simplify_eq. done. }
+  { intros ip Sn Hip sh skt bs sa Hsh Hskt.
+    rewrite insert_union_singleton_l in Hip.
+    apply lookup_union_Some in Hip; [|apply map_disjoint_dom; set_solver].
+    destruct Hip as [Hip|Hip].
+    - destruct (decide (ip = ipA)) as [->|Hneq]; last first.
+      { by rewrite lookup_insert_ne in Hip. }
+      rewrite lookup_insert in Hip.
+      simplify_eq.
+      destruct (decide (sh = shA)) as [->|Hneq]; last first.
+      { by rewrite lookup_insert_ne in Hsh. }
+      rewrite lookup_insert in Hsh. simplify_eq. set_solver.
+    - destruct (decide (ip = ipB)) as [->|Hneq]; last first.
+      { by rewrite lookup_insert_ne in Hip. }
+      rewrite lookup_insert in Hip.
+      simplify_eq.
+      destruct (decide (sh = shB)) as [->|Hneq]; last first.
+      { by rewrite lookup_insert_ne in Hsh. }
+      rewrite lookup_insert in Hsh. simplify_eq. set_solver. }
+  iIntros (Hinv) "!> Hunallocated Hrt Hlive Hσ _ Hfrag Hnode Hst".
+  iDestruct (unallocated_split with "Hunallocated") as "[HA HB]"; [set_solver|].
+  iMod (aneris_state_interp_socket_interp_allocate_singleton with "Hst [HB]")
+    as "[$ #HB]".
+  { rewrite /unallocated to_singletons_singleton. iApply "HB". }
+  iIntros "!>".
+  rewrite big_sepS_union; [|set_solver].
+  iDestruct "Hrt" as "[HrtA HrtB]".
+  rewrite !big_sepS_singleton.
+  rewrite /retransmit_live_roles=> /=.
+  iDestruct (live_roles_own_split with "Hlive") as "[HliveA HliveB]";
+    [set_solver|].
+  replace (dom {[ipA := ∅; ipB := ∅]}) with ({[ipA]} ∪ {[ipB]} : gset _)
+                                            by set_solver.
+  rewrite !big_sepS_union; [|set_solver..].
+  rewrite !big_sepS_singleton.
+  rewrite !lookup_total_insert.
+  rewrite !big_sepM_singleton.
+  simpl.
+  iDestruct "Hnode" as "[HnodeA HnodeB]".
+  iDestruct "Hσ" as "[[_ HshA] [_ HshB]]".
+  iSplitL "HrtA HnodeA HshA HliveA".
+  { iApply (wp_A with "[$HrtA $HshA $HliveA //]").
+    iIntros "!>" (v) "H".
+    iExists _. by iFrame. }
+  iSplitL "HrtB HnodeB HshB HliveB".
+  { iApply (wp_B with "[$HrtB $HshB $HliveB //]").
+    iIntros "!>" (v) "H".
+    iExists _. by iFrame. }
+  done.
+Qed.
